Introduce constant pointers (rough draft)

coq/DSigmaHCOL/ReifyProofs.v
@@ -45,8 +45,6 @@ Local Open Scope nat_scope.
 
 Import DSHCOLOnCarrierA.
 
-(*
-
 (* Type signatures of expressions as binary or unary functions with
 optional index *)
 
@@ -92,9 +90,9 @@ Class DSHBinCarrierA (a:AExpr) : Prop :=
 (* This relations represents consistent memory/envirnment combinations. That means all pointer variables should resolve to existing memory blocks *)
 Inductive EnvMemoryConsistent: evalContext -> memory -> Prop :=
 | EmptyEnvConsistent: forall m, EnvMemoryConsistent [] m
-| DSHPtrValConsistent: forall σ m a,
+| DSHPtrValConsistent: forall σ m n a,
     mem_block_exists a m ->
-    EnvMemoryConsistent σ m -> EnvMemoryConsistent (DSHPtrVal a :: σ) m
+    EnvMemoryConsistent σ m -> EnvMemoryConsistent (DSHPtrVal a n :: σ) m
 (* the remaining case does not depend on memory and just recurse over environment *)
 | DSHnatValConsistent : forall σ m n, EnvMemoryConsistent σ m -> EnvMemoryConsistent (DSHnatVal n :: σ) m
 | DSHCTypeValConsistent: forall σ m a, EnvMemoryConsistent σ m -> EnvMemoryConsistent (DSHCTypeVal a :: σ) m.
@@ -117,8 +115,9 @@ Lemma EnvMemoryConsistent_memory_lookup
       {mem : memory}
       {EC : EnvMemoryConsistent σ mem}
       (v : var_id)
+      (n : nat)
       (a : mem_block_id) :
-  List.nth_error σ v = Some (DSHPtrVal a) →
+  List.nth_error σ v = Some (DSHPtrVal a n) →
   is_Some (memory_lookup mem a).
 Proof.
   intros.
@@ -128,9 +127,10 @@ Proof.
     clear IHσ.
     cbn in H; some_inv.
     destruct a; inversion H; clear H; subst.
+    destruct H1.
     inversion EC; subst.
     apply memory_is_set_is_Some.
-    rewrite <-H2.
+    rewrite <-H0.
     assumption.
   -
     eapply IHσ.
@@ -161,15 +161,14 @@ Proof.
   inversion TC; subst d.
   unfold memory_lookup_err.
   assert (is_Some (memory_lookup mem a)).
-  eapply EnvMemoryConsistent_memory_lookup with (v0:=v).
+  eapply EnvMemoryConsistent_memory_lookup with (v0:=v) (n:=size).
   rewrite <-Heqo.
   reflexivity.
   apply is_Some_def in H; destruct H as [b H].
   rewrite H.
   constructor.
   Unshelve.
-  assumption.
-Qed.
+  assumption. Qed.
 
 Lemma evalNExpr_is_OK
       {σ: evalContext}
@@ -709,7 +708,8 @@ Proof.
   subst.
   destruct d0, d; inversion H4; try reflexivity.
   subst.
-  rewrite H5.
+  destruct H3.
+  rewrite H3.
   reflexivity.
 Qed.
 
@@ -1229,6 +1229,98 @@ Proof.
   apply H.
   apply kc.
 Qed.
+
+(* [DSHVal] is constant if it is a [DSHPtrVal] which points to a constant memory block (?) *)
+Definition is_const_ptr : DSHVal -> Prop. Admitted.
+
+(* ugly *)
+Inductive constants_match : evalContext -> relation memory :=
+| consistent_nil : forall mem0 mem1, constants_match [] mem0 mem1
+| consistent_const_cons : forall mem0 mem1 σ a size, is_const_ptr (DSHPtrVal a size) ->
+                                memory_lookup mem0 a = memory_lookup mem1 a ->
+                                constants_match ((DSHPtrVal a size) :: σ) mem0 mem1
+| consistent_nonconst_cons : forall mem0 mem1 σ v, not (is_const_ptr v) -> constants_match (v :: σ) mem0 mem1.
+
+(* [PVar i] is constant if it is a valid constant pointer *)
+Inductive PExpr_const (σ : evalContext) : PExpr -> Prop :=
+| PVar_const : forall i, opt_p is_const_ptr (List.nth_error σ i) -> PExpr_const σ (PVar i).
+
+Inductive MExpr_const (σ : evalContext) : MExpr -> Prop :=
+| MPtrDeref_const : forall p, PExpr_const σ p -> MExpr_const σ (MPtrDeref p)
+| MConst_const : forall b, MExpr_const σ (MConst b).
+                                              
+Inductive AExpr_const (σ : evalContext) : AExpr -> Prop :=
+| ANth_const   : forall m n,
+    MExpr_const σ m -> AExpr_const σ (ANth m n)
+| AVar_const   : forall n, AExpr_const σ (AVar n)
+| AConst_const : forall a, AExpr_const σ (AConst a)
+| AAbs_const   : forall a, AExpr_const σ a -> AExpr_const σ (AAbs a)
+| APlus_const  : forall a1 a2, AExpr_const σ a1 -> AExpr_const σ a2 -> AExpr_const σ (APlus  a1 a2)
+| AMinus_const : forall a1 a2, AExpr_const σ a1 -> AExpr_const σ a2 -> AExpr_const σ (AMinus a1 a2)
+| AMult_const  : forall a1 a2, AExpr_const σ a1 -> AExpr_const σ a2 -> AExpr_const σ (AMult  a1 a2)
+| AMin_const   : forall a1 a2, AExpr_const σ a1 -> AExpr_const σ a2 -> AExpr_const σ (AMin   a1 a2)
+| AMax_const   : forall a1 a2, AExpr_const σ a1 -> AExpr_const σ a2 -> AExpr_const σ (AMax   a1 a2)
+| AZless_const : forall a1 a2, AExpr_const σ a1 -> AExpr_const σ a2 -> AExpr_const σ (AZless a1 a2).
+
+Inductive DSHOperator_const (σ : evalContext) : DSHOperator -> Prop :=
+| DSHNop_const : DSHOperator_const σ DSHNop
+| DSHAssign_const : forall src dst, DSHOperator_const σ (DSHAssign src dst)
+| DSHIMap_const : forall n x_p y_p f, AExpr_const σ f -> DSHOperator_const σ (DSHIMap n x_p y_p f)
+| DSHBinOp_const : forall n x_p y_p f, AExpr_const σ f → DSHOperator_const σ (DSHBinOp n x_p y_p f)
+| DSHMemMap2_const : forall n x0_p x1_p y_p f, AExpr_const σ f → DSHOperator_const σ (DSHMemMap2 n x0_p x1_p y_p f)
+| DSHPower_const : forall n src dst f initial, AExpr_const σ f → DSHOperator_const σ (DSHPower n src dst f initial)
+| DSHLoop_const : forall n body, DSHOperator_const σ body -> DSHOperator_const σ (DSHLoop n body)
+| DSHAlloc_const : forall size body, DSHOperator_const σ body -> DSHOperator_const σ (DSHAlloc size body)
+| DSHMemInit_const : forall size y_p value, DSHOperator_const σ (DSHMemInit size y_p value)
+| DSHMemCopy_const : forall size x_p y_p, DSHOperator_const σ (DSHMemCopy size x_p y_p)
+| DSHSeq_const : forall f g, DSHOperator_const σ f → DSHOperator_const σ g → DSHOperator_const σ (DSHSeq f g).
+
+Lemma evalMexp_const `{MC : MExpr_const σ m} :
+  forall mem0 mem1,
+    constants_match σ mem0 mem1 ->
+    evalMexp mem0 σ m = evalMexp mem1 σ m.
+Admitted. (* a similar lemma was proven, but I lost the proof *) (* should be ok *)
+
+Lemma evalAexp_const `{AC : AExpr_const σ a} :
+  forall mem0 mem1,
+    constants_match σ mem0 mem1 ->
+    evalAexp mem0 σ a = evalAexp mem1 σ a.
+Proof.
+  intros.
+  dependent induction a.
+  (* base 1 *)
+  reflexivity.
+  (* base 2 *)
+  reflexivity.
+  (* base 3 *)
+  cbn.
+  inversion AC.
+  pose proof evalMexp_const mem0 mem1 (MC:=H1) H.
+  repeat break_match; try inl_inr; try constructor.
+  enough (Some c = Some c0) by (some_inv; assumption);
+    rewrite <-Heqo, <-Heqo0; inl_inr_inv; apply H3.
+  enough (Some c = None) by some_none;
+    rewrite <-Heqo, <-Heqo0; inl_inr_inv; apply H3.
+  enough (None = Some c) by some_none;
+    rewrite <-Heqo, <-Heqo0; inl_inr_inv; apply H3.
+  reflexivity.
+
+  (* inductive 1 *)
+  cbn.
+  assert (evalAexp mem0 σ a = evalAexp mem1 σ a) by (apply IHa; inversion AC; assumption).
+  repeat break_match; try inl_inr; [assumption | inl_inr_inv; rewrite H0; reflexivity].
+  (* inductive 2-7 *)
+  all: cbn.
+  all: assert (evalAexp mem0 σ a1 = evalAexp mem1 σ a1)
+    by (apply IHa1; inversion AC; assumption).
+  all: assert (evalAexp mem0 σ a2 = evalAexp mem1 σ a2)
+    by (apply IHa2; inversion AC; assumption).
+  all: repeat break_match; try inl_inr.
+  all: try assumption.
+  all: repeat inl_inr_inv; rewrite H0, H1; reflexivity.
+Qed.
+
+(*
 
 (* DSH expression as a "pure" function by enforcing the memory
    invariants guaranteeing that it depends only input memory block and
@@ -4746,5 +4838,4 @@ Proof.
     constructor.
    *)
 Admitted.
-
 *)
